split array type away from vprop

src/lowparse/LowParse.SteelST.ArrayPtr.fsti
@@ -1,110 +1,16 @@
 module LowParse.SteelST.ArrayPtr
+include LowParse.SteelST.ArrayPtr.Base
 
 open Steel.Memory
 open Steel.FractionalPermission
 module SZ = FStar.SizeT
 open Steel.ST.GenElim
 
-inline_for_extraction
-val t (t:Type u#0) : Type u#0
-
-[@@erasable]
-val array
-  (t: Type0)
-: Tot Type0
-
-val len
-  (#t: Type0)
-  (x: array t)
-: GTot SZ.t
-
-let length
-  (#t: Type0)
-  (x: array t)
-: GTot nat
-= SZ.v (len x)
-
-val array_perm
-  (#t: Type)
-  (x: array t)
-: GTot perm
-
-[@@erasable]
-val v (t: Type u#0) : Tot Type0
-
-val array_of (#a: _) (v: v a) : Tot (array a)
-val contents_of (#a: _) (v: v a) : GTot (Seq.lseq a (length (array_of v)))
-let contents_of' #a (v: v a) : GTot (Seq.seq a) =
-  contents_of v
-
-val array_contents_inj
-  (#a: _)
-  (v1 v2: v a)
-: Lemma
-  (requires (
-    array_of v1 == array_of v2 /\
-    contents_of v1 == contents_of v2
-  ))
-  (ensures (v1 == v2))
-  [SMTPatOr [
-    [SMTPat (array_of v1); SMTPat (array_of v2)];
-    [SMTPat (contents_of v1); SMTPat (contents_of v2)];
-  ]]
-
 val arrayptr
   (#a: Type0)
   (r: t a)
   ([@@@smt_fallback] value: v a)
 : Tot vprop
-
-val adjacent
-  (#t: Type0)
-  (x1 x2: array t)
-: Tot prop
-
-val merge
-  (#t: Type0)
-  (x1 x2: array t)
-: Ghost (array t)
-  (requires (adjacent x1 x2))
-  (ensures (fun y -> length y == length x1 + length x2 /\ array_perm y == array_perm x1 /\ array_perm y == array_perm x2))
-
-let adjacent_sizes_fit
-  (#t: Type0)
-  (x1 x2: array t)
-: Lemma
-  (requires (adjacent x1 x2))
-  (ensures (SZ.fits (length x1 + length x2)))
-  [SMTPat (adjacent x1 x2)]
-= let _ = merge x1 x2 in
-  ()
-
-let merge_into
-  (#t: Type0)
-  (x1 x2 y: array t)
-: Tot prop
-= adjacent x1 x2 /\
-  merge x1 x2 == y
-
-val merge_assoc
-  (#t: Type0)
-  (x1 x2 x3: array t)
-: Lemma
-  (requires (
-    (adjacent x1 x2 /\ adjacent x2 x3) \/
-    (adjacent x1 x2 /\ adjacent (merge x1 x2) x3) \/
-    (adjacent x2 x3 /\ adjacent x1 (merge x2 x3))
-  ))
-  (ensures (
-    adjacent x1 x2 /\ adjacent (merge x1 x2) x3 /\
-    adjacent x2 x3 /\ adjacent x1 (merge x2 x3) /\
-    merge (merge x1 x2) x3 == merge x1 (merge x2 x3)
-  ))
-  [SMTPatOr [
-    [SMTPat (adjacent x1 x2); SMTPat (adjacent x2 x3)];
-    [SMTPat (adjacent (merge x1 x2) x3)];
-    [SMTPat (adjacent x1 (merge x2 x3))];
-  ]]
 
 val join (#opened: _) (#a:Type) (#vl #vr: v a) (al ar:t a)
   : STGhost (v a) opened
@@ -115,13 +21,6 @@ val join (#opened: _) (#a:Type) (#vl #vr: v a) (al ar:t a)
             merge_into (array_of vl) (array_of vr) (array_of res) /\
             contents_of res == contents_of vl `Seq.append` contents_of vr
           )
-
-[@@noextract_to "krml"]
-let seq_slice
-  (#a:Type) (s:Seq.seq a) (i: nat) (j: nat) : Pure (Seq.seq a)
-  (requires (i <= j /\ j <= Seq.length s))
-  (ensures (fun _ -> True))
-= Seq.slice s i j
 
 val gsplit (#opened: _) (#a:Type) (#value: v a) (x: t a) (i:SZ.t)
   : STGhost (Ghost.erased (t a)) opened
@@ -192,40 +91,6 @@ val upd (#a:Type) (#value: v a) (r: t a) (i:SZ.t) (x:a)
                array_of value' == array_of value /\
                contents_of' value' == Seq.upd (contents_of' value) (SZ.v i) x
              )
-
-val set_array_perm
-  (#t: Type)
-  (a: array t)
-  (p: perm)
-: Ghost (array t)
-    (requires True)
-    (ensures (fun y -> len y == len a /\ array_perm y == p))
-
-val set_array_perm_idem
-  (#t: Type)
-  (a: array t)
-  (p1 p2: perm)
-: Lemma
-  (set_array_perm (set_array_perm a p1) p2 == set_array_perm a p2)
-  [SMTPat (set_array_perm (set_array_perm a p1) p2)]
-
-val set_array_perm_eq
-  (#t: Type)
-  (a: array t)
-: Lemma
-  (set_array_perm a (array_perm a) == a)
-  [SMTPat (set_array_perm a (array_perm a))]
-
-val set_array_perm_adjacent
-  (#t: Type)
-  (a1 a2: array t)
-  (p: perm)
-: Lemma
-  (requires (adjacent a1 a2))
-  (ensures (
-    merge_into (set_array_perm a1 p) (set_array_perm a2 p) (set_array_perm (merge a1 a2) p)
-  ))
-  [SMTPat (adjacent (set_array_perm a1 p) (set_array_perm a2 p))]
 
 val share
   (#opened: _)
