src/lowparse/steel_c_array/LowParse.SteelST.ArrayPtr.fst
@@ -1,31 +1,6 @@
 module LowParse.SteelST.ArrayPtr
+friend LowParse.SteelST.ArrayPtr.Base
 module STC = Steel.ST.C.Types
-
-let t elt = STC.array_ptr (STC.scalar elt)
-
-[@@erasable]
-noeq
-type array elt = {
-  array_ptr: STC.array (STC.scalar elt);
-  array_perm: Steel.FractionalPermission.perm;
-//  array_base_len: (len: SZ.t { SZ.v len == SA.base_len (STC.base (STC.array_ptr_of array_ptr)) });
-}
-
-let len x = SZ.uint_to_t (STC.array_length x.array_ptr)
-
-let array_perm x = x.array_perm
-
-[@@erasable]
-noeq
-type v t = {
-  v_array: array t;
-  v_contents: Seq.lseq t (length v_array);
-}
-
-let array_of x = x.v_array
-let contents_of x = x.v_contents
-
-let array_contents_inj _ _ = ()
 
 let mk_full_scalar_seq_index (#t: Type) (s: Seq.seq t) (i: nat { i < Seq.length s }) : GTot (STC.scalar_t t) =
   STC.mk_scalar (Seq.index s i)
@@ -50,19 +25,6 @@ let arrayptr0 (#elt: _) (r: t elt) (v: v elt) : Tot vprop =
   ))
 
 let arrayptr r v = arrayptr0 r v
-    
-let adjacent x1 x2 =
-  x1.array_perm == x2.array_perm /\
-  STC.array_ptr_of x2.array_ptr == STC.array_ref_shift (STC.array_ptr_of x1.array_ptr) (len x1)
-
-let merge x1 x2 = {
-  array_ptr = (| STC.array_ptr_of x1.array_ptr, Ghost.hide (len x1 `SZ.add` len x2) |);
-  array_perm = x1.array_perm;
-//  array_base_len = x1.array_base_len;
-}
-
-let merge_assoc x1 x2 x3 =
-  STC.array_ref_shift_assoc (STC.array_ptr_of x1.array_ptr) (len x1) (len x2)
 
 let join #_ #a #vl #vr al ar =
   rewrite (arrayptr al vl) (arrayptr0 al vl);
@@ -213,43 +175,6 @@ let upd #elt #v r i x =
   rewrite (STC.array_pts_to _ _) (arrayptr1 res s');
   rewrite (arrayptr0 r res) (arrayptr r res);
   return res
-
-let set_array_perm
-  (#t: Type)
-  (a: array t)
-  (p: perm)
-: Ghost (array t)
-    (requires True)
-    (ensures (fun y -> len y == len a /\ array_perm y == p))
-= {
-  a with array_perm = p
-}
-
-let set_array_perm_idem
-  (#t: Type)
-  (a: array t)
-  (p1 p2: perm)
-: Lemma
-  (set_array_perm (set_array_perm a p1) p2 == set_array_perm a p2)
-= ()
-
-let set_array_perm_eq
-  (#t: Type)
-  (a: array t)
-: Lemma
-  (set_array_perm a (array_perm a) == a)
-= ()
-
-let set_array_perm_adjacent
-  (#t: Type)
-  (a1 a2: array t)
-  (p: perm)
-: Lemma
-  (requires (adjacent a1 a2))
-  (ensures (
-    merge_into (set_array_perm a1 p) (set_array_perm a2 p) (set_array_perm (merge a1 a2) p)
-  ))
-= ()
 
 #set-options "--ide_id_info_off"
 
