src/lowparse/LowParse.SteelST.ArrayPtr.Base.fsti
@@ -1,0 +1,139 @@
+module LowParse.SteelST.ArrayPtr.Base
+open Steel.FractionalPermission
+module SZ = FStar.SizeT
+
+inline_for_extraction
+val t (t:Type u#0) : Type u#0
+
+[@@erasable]
+val array
+  (t: Type0)
+: Tot Type0
+
+val len
+  (#t: Type0)
+  (x: array t)
+: GTot SZ.t
+
+let length
+  (#t: Type0)
+  (x: array t)
+: GTot nat
+= SZ.v (len x)
+
+val array_perm
+  (#t: Type)
+  (x: array t)
+: GTot perm
+
+[@@erasable]
+val v (t: Type u#0) : Tot Type0
+
+val array_of (#a: _) (v: v a) : Tot (array a)
+val contents_of (#a: _) (v: v a) : GTot (Seq.lseq a (length (array_of v)))
+let contents_of' #a (v: v a) : GTot (Seq.seq a) =
+  contents_of v
+
+val array_contents_inj
+  (#a: _)
+  (v1 v2: v a)
+: Lemma
+  (requires (
+    array_of v1 == array_of v2 /\
+    contents_of v1 == contents_of v2
+  ))
+  (ensures (v1 == v2))
+  [SMTPatOr [
+    [SMTPat (array_of v1); SMTPat (array_of v2)];
+    [SMTPat (contents_of v1); SMTPat (contents_of v2)];
+  ]]
+
+val adjacent
+  (#t: Type0)
+  (x1 x2: array t)
+: Tot prop
+
+val merge
+  (#t: Type0)
+  (x1 x2: array t)
+: Ghost (array t)
+  (requires (adjacent x1 x2))
+  (ensures (fun y -> length y == length x1 + length x2 /\ array_perm y == array_perm x1 /\ array_perm y == array_perm x2))
+
+let adjacent_sizes_fit
+  (#t: Type0)
+  (x1 x2: array t)
+: Lemma
+  (requires (adjacent x1 x2))
+  (ensures (SZ.fits (length x1 + length x2)))
+  [SMTPat (adjacent x1 x2)]
+= let _ = merge x1 x2 in
+  ()
+
+let merge_into
+  (#t: Type0)
+  (x1 x2 y: array t)
+: Tot prop
+= adjacent x1 x2 /\
+  merge x1 x2 == y
+
+val merge_assoc
+  (#t: Type0)
+  (x1 x2 x3: array t)
+: Lemma
+  (requires (
+    (adjacent x1 x2 /\ adjacent x2 x3) \/
+    (adjacent x1 x2 /\ adjacent (merge x1 x2) x3) \/
+    (adjacent x2 x3 /\ adjacent x1 (merge x2 x3))
+  ))
+  (ensures (
+    adjacent x1 x2 /\ adjacent (merge x1 x2) x3 /\
+    adjacent x2 x3 /\ adjacent x1 (merge x2 x3) /\
+    merge (merge x1 x2) x3 == merge x1 (merge x2 x3)
+  ))
+  [SMTPatOr [
+    [SMTPat (adjacent x1 x2); SMTPat (adjacent x2 x3)];
+    [SMTPat (adjacent (merge x1 x2) x3)];
+    [SMTPat (adjacent x1 (merge x2 x3))];
+  ]]
+
+[@@noextract_to "krml"]
+let seq_slice
+  (#a:Type) (s:Seq.seq a) (i: nat) (j: nat) : Pure (Seq.seq a)
+  (requires (i <= j /\ j <= Seq.length s))
+  (ensures (fun _ -> True))
+= Seq.slice s i j
+
+val set_array_perm
+  (#t: Type)
+  (a: array t)
+  (p: perm)
+: Ghost (array t)
+    (requires True)
+    (ensures (fun y -> len y == len a /\ array_perm y == p))
+
+val set_array_perm_idem
+  (#t: Type)
+  (a: array t)
+  (p1 p2: perm)
+: Lemma
+  (set_array_perm (set_array_perm a p1) p2 == set_array_perm a p2)
+  [SMTPat (set_array_perm (set_array_perm a p1) p2)]
+
+val set_array_perm_eq
+  (#t: Type)
+  (a: array t)
+: Lemma
+  (set_array_perm a (array_perm a) == a)
+  [SMTPat (set_array_perm a (array_perm a))]
+
+val set_array_perm_adjacent
+  (#t: Type)
+  (a1 a2: array t)
+  (p: perm)
+: Lemma
+  (requires (adjacent a1 a2))
+  (ensures (
+    merge_into (set_array_perm a1 p) (set_array_perm a2 p) (set_array_perm (merge a1 a2) p)
+  ))
+  [SMTPat (adjacent (set_array_perm a1 p) (set_array_perm a2 p))]
