src/lowparse/steel_array/LowParse.SteelST.ArrayPtr.Base.fst
@@ -1,0 +1,78 @@
+module LowParse.SteelST.ArrayPtr.Base
+module SA = Steel.ST.Array
+
+let t elt = SA.ptr elt
+
+[@@erasable]
+noeq
+type array elt = {
+  array_ptr: SA.array elt;
+  array_perm: Steel.FractionalPermission.perm;
+  array_base_len: (len: SZ.t { SZ.v len == SA.base_len (SA.base (SA.ptr_of array_ptr)) });
+}
+
+let len x = SZ.uint_to_t (SA.length x.array_ptr)
+
+let array_perm x = x.array_perm
+
+[@@erasable]
+noeq
+type v t = {
+  v_array: array t;
+  v_contents: Seq.lseq t (length v_array);
+}
+
+let array_of x = x.v_array
+let contents_of x = x.v_contents
+
+let array_contents_inj _ _ = ()
+
+let adjacent x1 x2 =
+  x1.array_perm == x2.array_perm /\
+  SA.adjacent x1.array_ptr x2.array_ptr
+
+let merge x1 x2 = {
+  array_ptr = SA.merge x1.array_ptr x2.array_ptr;
+  array_perm = x1.array_perm;
+  array_base_len = x1.array_base_len;
+}
+
+let merge_assoc x1 x2 x3 =
+  SA.merge_assoc x1.array_ptr x2.array_ptr x3.array_ptr
+
+let set_array_perm
+  (#t: Type)
+  (a: array t)
+  (p: perm)
+: Ghost (array t)
+    (requires True)
+    (ensures (fun y -> len y == len a /\ array_perm y == p))
+= {
+  a with array_perm = p
+}
+
+let set_array_perm_idem
+  (#t: Type)
+  (a: array t)
+  (p1 p2: perm)
+: Lemma
+  (set_array_perm (set_array_perm a p1) p2 == set_array_perm a p2)
+= ()
+
+let set_array_perm_eq
+  (#t: Type)
+  (a: array t)
+: Lemma
+  (set_array_perm a (array_perm a) == a)
+= ()
+
+let set_array_perm_adjacent
+  (#t: Type)
+  (a1 a2: array t)
+  (p: perm)
+: Lemma
+  (requires (adjacent a1 a2))
+  (ensures (
+    merge_into (set_array_perm a1 p) (set_array_perm a2 p) (set_array_perm (merge a1 a2) p)
+  ))
+= ()
